ems/Skeleton.v
@@ -1,77 +1,42 @@
-Require Import Coqlib.
 Require Export ZArith.
 Require Import String.
-Require Import PCM.
-Require Export AList.
+Require Import Orders.
 
-Set Implicit Arguments.
+(* one instance per lang *)
+Module Sk.
 
-Local Open Scope nat_scope.
+  Class ld: Type := mk {
+    t:> Type;
+    unit: t;
+    add: t -> t -> t;
+    canon: t -> t;
+    wf: t -> Prop;
+    le: t -> t -> Prop;
+    le_PreOrder:> PreOrder le;
+    le_canon: forall a, le a (canon a);
+    le_canon_rev: forall a, le (canon a) a;
+    add_comm: forall a b (WF: wf (add a b)),
+        canon (add a b) = canon (add b a);
+    add_assoc: forall a b c, add a (add b c) = add (add a b) c;
+    add_unit_l: forall a, add unit a = a;
+    add_unit_r: forall a, add a unit = a;
+    le_add_l: forall a b, le a (add b a);
+    le_add_r: forall a b, le a (add a b);
+    wf_comm: forall a b, wf (add a b) -> wf (add b a);
+    wf_canon: forall a, wf a -> wf (canon a);
+    unit_wf: wf unit;
+    wf_mon: forall a b, wf (canon (add a b)) -> wf (canon a);
+    extends := fun a b => exists ctx, canon (add a ctx) = b;
+  }
+  .
+
+End Sk.
 
 Notation gname := string (only parsing). (*** convention: not capitalized ***)
 Notation mname := string (only parsing). (*** convention: capitalized ***)
 
-
-Fixpoint _find_idx {A} (f: A -> bool) (l: list A) (acc: nat): option (nat * A) :=
-  match l with
-  | [] => None
-  | hd :: tl => if (f hd) then Some (acc, hd) else _find_idx f tl (S acc)
-  end
-.
-
-Definition find_idx {A} (f: A -> bool) (l: list A): option (nat * A) := _find_idx f l 0.
-
-Notation "'do' ' X <- A ; B" := (o_bind A (fun _x => match _x with | X => B end))
-                                  (at level 200, X pattern, A at level 100, B at level 200)
-                                : o_monad_scope.
-
-Lemma find_idx_red {A} (f: A -> bool) (l: list A):
-  find_idx f l =
-  match l with
-  | [] => None
-  | hd :: tl =>
-    if (f hd)
-    then Some (0%nat, hd)
-    else
-      do (n, a) <- find_idx f tl;
-      Some (S n, a)
-  end.
-Proof.
-  unfold find_idx. generalize 0. induction l; ss.
-  i. des_ifs; ss.
-  - rewrite Heq0. ss.
-  - rewrite Heq0. specialize (IHl (S n)). rewrite Heq0 in IHl. ss.
-Qed.
-
-
-Lemma NoDup_map A B (f: A -> B) l
-  :
-    NoDup l -> ((forall a b, a<>b -> In a l -> In b l -> f a <> f b) <-> NoDup (map f l)).
-Proof.
-  i. split; i.
-  - revert H0. induction H; i; ss.
-    + econs.
-    + econs.
-      * red. i. apply H.
-        assert (forall a, In a l -> f x <> f a).
-        { i. apply H1; et. red. i. clarify. }
-        clear - H2 H3. 
-        revert_until l. induction l; i; ss.
-        hexploit (H3 a); et. i. des; clarify.
-        { rewrite H2 in H. clarify. }
-        right. apply IHl; et.
-      * apply IHNoDup. i. apply H1; et. 
-  - revert_until l. induction l; i; ss.
-    des; clarify.
-    + apply in_map with (f := f) in H2. inv H0. clear - H2 H5.
-      red. i. apply H5. rewrite <- H. et.
-    + apply in_map with (f := f) in H3. inv H0. clear - H3 H5.
-      red. i. apply H5. rewrite H. et.
-    + inv H. inv H0. apply IHl; et. 
-Qed.
-
+(* auxilary structure to interpret sk as initial global env *)
 Module SkEnv.
-
   Notation mblock := nat (only parsing).
   Notation ptrofs := Z (only parsing).
 
@@ -83,343 +48,4 @@ Module SkEnv.
 
   Definition wf (ske: t): Prop :=
     forall id blk, ske.(id2blk) id = Some blk <-> ske.(blk2id) blk = Some id.
-
 End SkEnv.
-
-
-Require Import Orders.
-Require Import PCM.
-From compcert Require Import Maps Clightdefs.
-
-Module Sk.
-  Class ld: Type := mk {
-    t:> Type;
-    sem: Type;
-    unit: t;
-    add: t -> t -> t;
-    canon: t -> sem;
-    wf: sem -> Prop;
-    add_comm: forall a b,
-      canon (add a b) = canon (add b a);
-    add_assoc: forall a b c,
-      canon (add a (add b c)) = canon (add (add a b) c);
-    add_unit_l: forall a, canon (add unit a) = canon a;
-    add_unit_r: forall a, canon (add a unit) = canon a;
-    (* wf_comm: forall a b, wf (add a b) -> wf (add b a);
-    wf_assoc: forall a b c, wf (add a (add b c)) <-> wf (add (add a b) c); *)
-    add_canon: forall a b a' b',
-      canon a = canon a' ->
-        canon b = canon b' ->
-          canon (add a b) = canon (add a' b');
-    unit_wf: wf (canon unit);
-    wf_mon: forall a b, wf (canon (add a b)) -> wf (canon a);
-    extends := fun a b => exists ctx, canon (add a ctx) = canon b;
-  }
-  .
-
-  Section SK.
-  Context {M: RA.t}.
-
-  Definition _add : option RA.car -> option RA.car -> option RA.car :=
-    fun optx opty =>
-      match optx, opty with
-      | Some x, Some y => Some (RA.add x y)
-      | Some x, None => Some x
-      | None, Some y => Some y
-      | None, None => None
-      end.
-
-  Program Instance globalenv : ld := {
-    t := PTree.t RA.car;
-    sem := alist positive RA.car;
-    unit := PTree.empty RA.car;
-    add := PTree.combine _add;
-    canon:= @PTree.elements RA.car;
-    wf := fun m => (forall s x, alist_find s m = Some x -> RA.wf x)
-                   /\ NoDup (map (string_of_ident ∘ fst) m);
-  }.
-  Next Obligation.
-  Proof.
-    unfold add. erewrite PTree.combine_commut; et.
-    i. unfold _add. des_ifs. f_equal. apply RA.add_comm. 
-  Qed.
-  Next Obligation.
-  Proof.
-    apply PTree.elements_extensional.
-    i. repeat (rewrite PTree.gcombine; et).
-    unfold _add. des_ifs. f_equal. apply RA.add_assoc.
-  Qed.
-  Next Obligation.
-  Proof.
-    apply PTree.elements_extensional.
-    i. rewrite PTree.xgcombine_r; et.
-    unfold _add. des_ifs.
-  Qed.
-  Next Obligation.
-  Proof.
-    apply PTree.elements_extensional.
-    i. repeat (rewrite PTree.gcombine; et).
-    unfold _add. des_ifs.
-    all: rewrite PTree.gempty in Heq0; clarify.
-  Qed.
-  Next Obligation.
-  Proof.
-    apply PTree.elements_extensional.
-    i. repeat (rewrite PTree.gcombine; et).
-    replace (a ! i) with (a' ! i); cycle 1.
-    2: f_equal.
-    - destruct (a ! i) eqn: E; destruct (a' ! i) eqn: E1; et.
-      + f_equal. apply PTree.elements_correct in E.
-        apply PTree.elements_correct in E1.
-        rewrite H in E. pose proof (PTree.elements_keys_norepet a).
-        rewrite H in H1.
-        set (PTree.elements a') in *. clearbody l. clear - E E1 H1.
-        revert_until l. induction l; i; ss. des; clarify; ss.
-        * inv H1. eapply in_map with (f:=fst) in E. clarify.
-        * inv H1. eapply in_map with (f:=fst) in E1. clarify.
-        * eapply IHl; et. inv H1. et.
-      + apply PTree.elements_correct in E.
-        rewrite H in E.
-        apply PTree.elements_complete in E.
-        clarify.
-      + apply PTree.elements_correct in E1.
-        rewrite <- H in E1.
-        apply PTree.elements_complete in E1.
-        clarify.
-    - destruct (b ! i) eqn: E; destruct (b' ! i) eqn: E1; et.
-      + f_equal. apply PTree.elements_correct in E.
-        apply PTree.elements_correct in E1.
-        rewrite H0 in E. pose proof (PTree.elements_keys_norepet b).
-        rewrite H0 in H1.
-        set (PTree.elements b') in *. clearbody l. clear - E E1 H1.
-        revert_until l. induction l; i; ss. des; clarify; ss.
-        * inv H1. eapply in_map with (f:=fst) in E. clarify.
-        * inv H1. eapply in_map with (f:=fst) in E1. clarify.
-        * eapply IHl; et. inv H1. et.
-      + apply PTree.elements_correct in E.
-        rewrite H0 in E.
-        apply PTree.elements_complete in E.
-        clarify.
-      + apply PTree.elements_correct in E1.
-        rewrite <- H0 in E1.
-        apply PTree.elements_complete in E1.
-        clarify.
-  Qed.
-  Next Obligation.
-  Proof.
-    split; clarify. econs.
-  Qed.
-  Next Obligation.
-  Proof.
-    split.
-    - i.
-      assert (alist_find s (PTree.elements (PTree.combine _add a b)) = _add (Some x) (b ! s)).
-      { i. apply alist_find_some in H1.
-        apply PTree.elements_complete in H1.
-        destruct (b ! s) eqn: E; eapply alist_find_some_iff.
-        1,3: rewrite CoqlibC.NoDup_norepet; apply PTree.elements_keys_norepet.
-        all: apply PTree.elements_correct; rewrite PTree.gcombine; et; rewrite H1, E; ss. }
-      destruct (b ! s); ss; hexploit H; et. apply RA.wf_mon.
-    - rewrite <- map_map. 
-      rewrite <- NoDup_map.
-      2: rewrite CoqlibC.NoDup_norepet; apply PTree.elements_keys_norepet.
-      i. rewrite <- map_map in H0.
-      rewrite <- NoDup_map in H0.
-      2: rewrite CoqlibC.NoDup_norepet; apply PTree.elements_keys_norepet.
-      apply H0; et.
-      + rewrite in_map_iff in H2. des. destruct x. clarify.
-        apply PTree.elements_complete in H4. 
-        rewrite in_map_iff; ss.
-        destruct (b ! p) eqn: E.
-        * eexists (p, _). split; et.
-          apply PTree.elements_correct.
-          rewrite PTree.gcombine; et. rewrite H4, E. et.
-        * eexists (p, _). split; et.
-          apply PTree.elements_correct.
-          rewrite PTree.gcombine; et. rewrite H4, E. et.
-      + rewrite in_map_iff in H3. des. destruct x. clarify.
-        apply PTree.elements_complete in H4. 
-        rewrite in_map_iff; ss.
-        destruct (b ! p) eqn: E.
-        * eexists (p, _). split; et.
-          apply PTree.elements_correct.
-          rewrite PTree.gcombine; et. rewrite H4, E. et.
-        * eexists (p, _). split; et.
-          apply PTree.elements_correct.
-          rewrite PTree.gcombine; et. rewrite H4, E. et.
-  Qed.
-
-  Local Existing Instance globalenv.
-
-  (*** TODO: It might be nice if Sk.t also constitutes a resource algebra ***)
-  (*** At the moment, List.app is not assoc/commutative. We need to equip RA with custom equiv. ***)
-
-  Definition load_skenv (sks: sem): (SkEnv.t) :=
-    {|
-      SkEnv.blk2id := fun blk => do '(id, _) <- (List.nth_error sks blk); Some (string_of_ident id);
-      SkEnv.id2blk := fun gn => do '(blk, _) <- find_idx (fun '(id', _) => dec gn (string_of_ident id')) sks; Some blk
-    |}
-  .
-
-  Lemma load_skenv_wf
-        sks
-        (WF: wf sks)
-    :
-      <<WF: SkEnv.wf (load_skenv sks)>>
-  .
-  Proof.
-    red. ss. des. split; i; ss.
-    - uo. des_ifs.
-      + assert (id = string_of_ident (fst p1)).
-        { clear - Heq1. revert_until sks. induction sks; ss; i.
-          rewrite find_idx_red in Heq1. uo. des_ifs.
-          - destruct dec; clarify.
-          - destruct p. ss. eapply IHsks; et. } 
-        assert (p1 = (p0, c)).
-        { clear -Heq1 Heq0. revert_until sks. induction sks; ss; i.
-          rewrite find_idx_red in Heq1. uo. des_ifs.
-          - destruct dec; ss; clarify.
-          - destruct p. ss. eapply IHsks; et. }
-        clarify.
-      + exfalso. clear -Heq2 Heq0.
-        revert_until sks. induction sks; i; ss.
-        rewrite find_idx_red in Heq2. uo. des_ifs.
-        destruct p. ss. eapply IHsks; et.
-    - uo. des_ifs.
-      + clear - WF0 Heq1 Heq0. revert_until sks. induction sks; i; ss.
-        rewrite find_idx_red in Heq0. uo. des_ifs.
-        * destruct dec; clarify. ss.
-          inv WF0. destruct blk; et.
-          ss. apply Coqlib.nth_error_in in Heq1.
-          apply in_map with (f:=fst) in Heq1.
-          ss. apply in_map with (f:=string_of_ident) in Heq1.
-          rewrite map_map in Heq1. rewrite e in Heq1. clarify.
-        * destruct blk; ss; clarify.
-          { destruct dec; clarify. }
-          assert (Some (fst p) = Some blk); clarify.
-          inv WF0. destruct p.
-          eapply IHsks; et. 
-      + exfalso. clear -Heq2 Heq0.
-        revert_until sks. induction sks; i; ss.
-        * destruct blk; clarify.
-        * rewrite find_idx_red in Heq0. uo. des_ifs.
-          destruct blk; ss; clarify.
-          { destruct dec; clarify. }
-          eapply IHsks; et.
-  Qed.
-
-  Program Instance incl_PreOrder: PreOrder extends.
-  Next Obligation.
-  Proof.
-    ii. unfold extends. eexists unit. apply add_unit_r.
-  Qed.
-  Next Obligation.
-  Proof.
-    ii. unfold extends in *. des. 
-    exists (add ctx0 ctx). rewrite add_assoc.
-    rewrite <- H0.
-    apply add_canon; et.
-  Qed.
-
-  (* Lemma sort_incl sk
-    :
-      incl sk (sort sk).
-  Proof.
-    ii. eapply Permutation.Permutation_in; [|apply IN].
-    eapply SkSort.sort_permutation.
-  Qed.
-
-  Lemma sort_incl_rev sk
-    :
-      incl (sort sk) sk.
-  Proof.
-    ii. eapply Permutation.Permutation_in; [|apply IN].
-    symmetry. eapply SkSort.sort_permutation.
-  Qed. *)
-
-  Definition incl_env (sk0: Sk.t) (skenv: SkEnv.t): Prop :=
-    forall gn gd (IN: sk0 ! (ident_of_string gn) = Some gd),
-    exists blk, <<FIND: skenv.(SkEnv.id2blk) gn = Some blk>>.
-
-  Lemma incl_incl_env sk0 sk1
-        (INCL: extends sk0 sk1)
-    :
-      incl_env sk0 (load_skenv (canon sk1)).
-  Proof.
-    ii. unfold extends in *. des. rewrite <- INCL.
-    ss. uo. des_ifs; et.
-    exfalso. clear - IN Heq0.
-    apply PTree.elements_correct in IN.
-    apply in_map with (f:=fst) in IN. ss.
-    assert (~ In (ident_of_string gn) (map fst (PTree.elements (PTree.combine _add sk0 ctx)))).
-    { clear IN. set (PTree.elements _) in *. clearbody l.
-      move l at top. revert_until l. induction l; i; ss.
-      red. i. des.
-      - rewrite find_idx_red in Heq0. uo. des_ifs.
-        ss. clarify. rewrite string_of_ident_of_string in Heq.
-        destruct dec; clarify.
-      - rewrite find_idx_red in Heq0. uo. des_ifs.
-        eapply IHl; et. }
-    clear Heq0. apply H. clear H.
-    apply in_map_iff. apply in_map_iff in IN.
-    des. destruct x. ss. clarify. apply PTree.elements_complete in IN0.
-    destruct (ctx ! (ident_of_string gn)) eqn: E.
-    - eexists (_, _). split; et. apply PTree.elements_correct.
-      rewrite PTree.gcombine; et. rewrite IN0, E. ss.
-    - eexists (_, _). split; et. apply PTree.elements_correct.
-      rewrite PTree.gcombine; et. rewrite IN0, E. ss.
-  Qed.
-
-  Lemma in_env_in_sk :
-    forall sk blk symb
-      (FIND: SkEnv.blk2id (load_skenv (canon sk)) blk = Some symb),
-    exists id def, string_of_ident id = symb /\ sk ! id = Some def.
-  Proof.
-    i. ss. uo. des_ifs. apply Coqlib.nth_error_in in Heq0.
-    apply PTree.elements_complete in Heq0. et.
-  Qed.
-
-  Lemma in_sk_in_env :
-    forall sk def gn
-           (IN: sk ! (ident_of_string gn) = Some def),
-    exists blk, SkEnv.blk2id (load_skenv (canon sk)) blk = Some gn.
-  Proof.
-    i. ss. apply PTree.elements_correct in IN.
-    apply In_nth_error in IN. des. exists n. rewrite IN.
-    uo. rewrite string_of_ident_of_string. et.
-  Qed.
-
-  Lemma env_range_some :
-    forall sks blk
-      (BLKRANGE : blk < Datatypes.length sks),
-      <<FOUND : exists symb, SkEnv.blk2id (load_skenv sks) blk = Some symb>>.
-  Proof.
-    ss. i. red. uo. des_ifs; et.
-    apply nth_error_None in Heq0. nia.
-  Qed.
-
-  Lemma env_found_range :
-    forall sks symb blk
-      (FOUND : SkEnv.id2blk (load_skenv sks) symb = Some blk),
-      <<BLKRANGE : blk < Datatypes.length sks>>.
-  Proof.
-    i. ss. uo. des_ifs. red. revert_until sks.
-    induction sks; i; ss; clarify.
-    rewrite find_idx_red in Heq0. uo. des_ifs; try nia.
-    assert (fst p < List.length sks); try nia.
-    destruct p. eapply IHsks; et.
-  Qed.
-
-  Lemma sk_incl_gd (sk0 sk1: t) gn blk gd: 
-    Sk.extends sk0 sk1 ->
-    SkEnv.id2blk (load_skenv (Maps.PTree.elements sk1)) gn = Some blk ->
-    Maps.PTree.get (ident_of_string gn) sk0 = Some gd ->
-    nth_error (Maps.PTree.elements sk1) blk = Some (ident_of_string gn, gd).
-  Proof.
-  Admitted.
-
-
-
-End SK.
-
-End Sk.
